Values.v
@@ -25,3 +25,14 @@ Module Mem.
   Definition write (m : t) (p : ptr) (x : memdata) : t :=
     fset ptr_eq p x m.
 End Mem.
+
+(* Functions and signatures *)
+
+Definition fid : Set := nat.
+
+Record f_sig := mk_f_sig {
+  f_arg_t : Type;
+  f_ret_t : Type;
+}.
+
+Definition sig_context := fid -> option f_sig.
